\documentclass[a4paper]{article}

\usepackage{latexsym,a4wide}

% The definition of \ifundefined is exercise 7.7 in the \TeX book
% \csname <Tokens> \endcsname is essentially \<Tokens>, i.e.
% some kind of evaluation. However, <Tokens> may contain tex-commands
% that are evaluated.
% \relax does nothing. Does this mean that \ifx\csname#1\endcsname
% is not evaluated when defining \ifundefined ?
% \expandafter evaluates everything after \ifx and then puts \ifx
% again in front.
% \ifndef{x}{y} tests whether x is defined. If yes, \x is carried out
% (the else part \csname#1\endcsname) otherwise y is the result.
% \ifdef{x} does \x if defined, nothing otherwise
\def\ifundefined#1{\expandafter\ifx\csname#1\endcsname\relax}
\newcommand{\ifndef}[2]{\ifundefined{#1}{#2}\else{\csname#1\endcsname}\fi}
\newcommand{\ifdef}[1]{\ifndef{#1}{}}

\newenvironment{fma}%
{\begin{equation}\begin{minipage}{0.85\linewidth}\raggedright}%
{\end{minipage}\end{equation}}

\newcommand{\udo}{$\langle$}
\newcommand{\udc}{$\rangle$}
\newcommand{\ubo}{$[$}
\newcommand{\ubc}{$]$}
\newcommand{\mkdia}[1]{\mbox{$\langle$#1$\rangle$}}
\newcommand{\mkbox}[1]{\mbox{$[$#1$]$}}
\newcommand{\tildesym}{\raisebox{-4pt}{\bf\~{}}}
\newcommand{\hatsym}{\mbox{\bf\^{} }}

\newcommand{\Fol}{\mbox{$\vdash\ $}}
\newcommand{\Not}{\mbox{$\neg\ $}}
\newcommand{\And}{\mbox{$\wedge\ $}}
\newcommand{\Or}{\mbox{$\vee\ $}}
\newcommand{\Imp}{\mbox{$\rightarrow\ $}}
\newcommand{\Equiv}{\mbox{$\leftrightarrow\ $}}
\newcommand{\All}{\mbox{$\forall\ $}}
\newcommand{\Ex}{\mbox{$\exists\ $}}

\newcommand{\tab}[1]{\mbox{$\phantom{\mbox{#1}}$}}
\newcommand{\tabx}[1]{\hspace*{#1ex}}
\newcommand{\tabif}{\tab{{\bf if}}}
\newcommand{\tabbe}{\tab{{\bf be}}}
\newcommand{\taball}{\mbox{$\phantom{\forall\ }$}}
\newcommand{\tabex}{\mbox{$\phantom{\exists\ }$}}
\newcommand{\taba}{\mbox{$\phantom{\wedge\ }$}}
\newcommand{\tabbo}{\mbox{$\phantom{(}$}}
\newcommand{\tabe}{\mbox{$\phantom{\leftrightarrow\ }$}}
\newcommand{\tabi}{\mbox{$\phantom{\rightarrow\ }$}}
\newcommand{\tabn}{\mbox{$\phantom{\neg\ }$}}
\newcommand{\tabo}{\mbox{$\phantom{\vee\ }$}}
\newcommand{\tabf}{\mbox{$\phantom{\vdash\ }$}}
\newcommand{\tabudo}{\mbox{$\phantom{\langle}$}}
\newcommand{\tabudc}{\mbox{$\phantom{\langle\ }$}}
\newcommand{\tabubo}{\mbox{$\phantom{[}$}}
\newcommand{\tabubc}{\mbox{$\phantom{]\ }$}}


\parindent0cm
\pagestyle{myheadings}
\markright{eq}

\begin{document}
\raggedright
              



\begin{minipage}{\textwidth}
\begin{center}
\input{eq-tree}
\end{center}
\end{minipage}

\vspace{5ex}

{\Huge eq}

\vspace{5ex}

 \Fol k $\neq$ 0 \Imp (m $*$ k = n $*$ k \Equiv m = n)

\begin{itemize}
\item proofsteps: 6
\item interactions: 2
\item automation: 66.6 \%
\item used lemmas: rsucc-01, zero-01, zero, mult-c, mult-a 
\item used simplifier rules:
n $\neq$ 0 \Fol m = n -1 \Equiv n = m +1 (elim)

 \Fol m + n = m + $\mbox{n}_{0}$ \Equiv n = $\mbox{n}_{0}$

 \Fol m + n = 0 \Equiv m = 0 \And n = 0

 \Fol m + n = n + m

 \Fol (m + $\mbox{n}_{0}$) + $\mbox{n}_{1}$ = m + $\mbox{n}_{0}$ + $\mbox{n}_{1}$

 \Fol m +1 = m + 1



               \end{itemize}



\vspace{3ex}\rule{1\textwidth}{1mm}


1) simplifier: simplifier \\
 \Fol k $\neq$ 0 \Imp (m $*$ k = n $*$ k \Equiv m = n)

\vspace{-1.5ex}\_\hrulefill \_

$\bullet$2) lemma mult-a \\
 \Fol k $*$ m $*$ n = (k $*$ m) $*$ n

\vspace{-1.5ex}\_\hrulefill \_

$\bullet$3)  (from 1) lemma mult-c \\
 \Fol m $*$ n = n $*$ m

\vspace{-1.5ex}\_\hrulefill \_

4)  (from 1) Interactive: structural induction  for m\\
m $*$ k = n $*$ k \Fol k = 0, m = n

\vspace{-1.5ex}\_\hrulefill \_

$\bullet$5) lemma mult-a \\
 \Fol k $*$ m $*$ n = (k $*$ m) $*$ n

\vspace{-1.5ex}\_\hrulefill \_

$\bullet$6)  (from 4) lemma mult-c \\
 \Fol m $*$ n = n $*$ m

\vspace{-1.5ex}\_\hrulefill \_

$\bullet$7)  (from 4) lemma zero \\
 \Fol 0 $*$ n = 0

\vspace{-1.5ex}\_\hrulefill \_

$\bullet$8)  (from 4) lemma zero-01 \\
 \Fol k $*$ m = 0 \Equiv k = 0 \Or m = 0

\vspace{-1.5ex}\_\hrulefill \_

9)  (from 4) simplifier: simplifier \\
\All k, $\mbox{n}_{0}$. n $*$ k = $\mbox{n}_{0}$ $*$ k \Imp k = 0 \Or n = $\mbox{n}_{0}$ \Fol n +1 $*$ k = $\mbox{n}_{0}$ $*$ k \Imp k = 0 \Or n +1 = $\mbox{n}_{0}$

\vspace{-1.5ex}\_\hrulefill \_

$\bullet$10) lemma mult-a \\
 \Fol k $*$ m $*$ n = (k $*$ m) $*$ n

\vspace{-1.5ex}\_\hrulefill \_

$\bullet$11)  (from 9) lemma mult-c \\
 \Fol m $*$ n = n $*$ m

\vspace{-1.5ex}\_\hrulefill \_

$\bullet$12)  (from 9) lemma rsucc-01 \\
 \Fol (m + 1) $*$ n = m $*$ n + n

\vspace{-1.5ex}\_\hrulefill \_

13)  (from 9) Interactive: all left  2 with k, $\mbox{n}_{0}$ -1\\
n $*$ k + k = $\mbox{n}_{0}$ $*$ k, \All k, $\mbox{n}_{0}$. n $*$ k = $\mbox{n}_{0}$ $*$ k \Imp k = 0 \Or n = $\mbox{n}_{0}$ \Fol k = 0, n + 1 = $\mbox{n}_{0}$

\vspace{-1.5ex}\_\hrulefill \_

14) simplifier: simplifier \\
\tabf n $*$ k + k = $\mbox{n}_{0}$ $*$ k, n $*$ k = $\mbox{n}_{0}$ -1 $*$ k \Imp k = 0 \Or n = $\mbox{n}_{0}$ -1, \\
 \tabf \All k, $\mbox{n}_{0}$. n $*$ k = $\mbox{n}_{0}$ $*$ k \Imp k = 0 \Or n = $\mbox{n}_{0}$ \\
\Fol k = 0, n + 1 = $\mbox{n}_{0}$

\vspace{-1.5ex}\_\hrulefill \_

15) elimination: insert elim lemma  elim-pred-c from nat-basic1\\
n $\leftarrow$ $\mbox{n}_{0}$, m $\leftarrow$ m\\
\tabf n $*$ k + k = $\mbox{n}_{0}$ $*$ k, \All k, $\mbox{n}_{0}$. n $*$ k = $\mbox{n}_{0}$ $*$ k \Imp k = 0 \Or n = $\mbox{n}_{0}$, n $*$ k = $\mbox{n}_{0}$ -1 $*$ k \Imp n = $\mbox{n}_{0}$ -1 \\
\Fol k = 0, n + 1 = $\mbox{n}_{0}$

\vspace{-1.5ex}\_\hrulefill \_

$\bullet$16) lemma mult-a \\
 \Fol k $*$ m $*$ n = (k $*$ m) $*$ n

\vspace{-1.5ex}\_\hrulefill \_

$\bullet$17)  (from 15) lemma mult-c \\
 \Fol m $*$ n = n $*$ m

\vspace{-1.5ex}\_\hrulefill \_

$\bullet$18)  (from 15) lemma zero \\
 \Fol 0 $*$ n = 0

\vspace{-1.5ex}\_\hrulefill \_

$\bullet$19)  (from 15) lemma mult-a \\
 \Fol k $*$ m $*$ n = (k $*$ m) $*$ n

\vspace{-1.5ex}\_\hrulefill \_

$\bullet$20)  (from 15) lemma mult-c \\
 \Fol m $*$ n = n $*$ m

\vspace{-1.5ex}\_\hrulefill \_

$\bullet$21)  (from 15) lemma rsucc-01 \\
 \Fol (m + 1) $*$ n = m $*$ n + n

\vspace{-1.5ex}\_\hrulefill \_



\end{document}

