\documentclass[a4paper]{article}

\usepackage{latexsym,a4wide,logicdefs}

\parindent0cm


\begin{document}
\raggedright
              
Pot2-zero:\\\tab{xxx} \Fol 2$\hatsym$ 0 = 1

Pot2-succ:\\\tab{xxx} \Fol 2$\hatsym$ n +1 = 2 $*$ 2$\hatsym$ n

Log2def:\\\tab{xxx} \Fol 2$\hatsym$ m $\le$ n \And n $<$ 2$\hatsym$ m +1 \Imp $\mbox{log}_{2}$ n = m

Logdef:\\\tab{xxx} \Fol m $\hatsym$ \Var{n}{0} $\le$ n \And n $<$ m $\hatsym$ \Var{n}{0} +1 \Imp log(m, n) = \Var{n}{0}

Pot-succ:\\\tab{xxx} \Fol n $\hatsym$ m +1 = n $\hatsym$ m $*$ n

Pot-zero:\\\tab{xxx} \Fol n $\hatsym$ 0 = 1

add:\\\tab{xxx} \Fol m $\hatsym$ (n + \Var{n}{0}) = m $\hatsym$ n $*$ m $\hatsym$ \Var{n}{0}

inj:\\\tab{xxx} \Fol 2$\hatsym$ n = 2$\hatsym$ m \Equiv n = m

inj-02:\\\tab{xxx} \Fol 2$\hatsym$ n = 2 $*$ 2$\hatsym$ m \Equiv n = m + 1

ladd:\\\tab{xxx}m $\neq$ 0 \Fol \Not $\mbox{log}_{2}$(m + n) $<$ $\mbox{log}_{2}$ m

ladd-01:\\\tab{xxx}n $\neq$ 0 \Fol m = n + \Var{n}{0} \Imp \Not $\mbox{log}_{2}$ m $<$ $\mbox{log}_{2}$ n

lemma-ax2:\\\tab{xxx} \Fol 2$\hatsym$(n + 1) = 2 $*$ 2$\hatsym$ n

lls:\\\tab{xxx} \Fol n $\neq$ 0 \Imp \Not n $<$ 2$\hatsym$ $\mbox{log}_{2}$ n

lls-01:\\\tab{xxx} \Fol n $<$ 2$\hatsym$($\mbox{log}_{2}$ n + 1)

lls-02:\\\tab{xxx}n $\neq$ 0 \Fol $\mbox{log}_{2}$ m $<$ $\mbox{log}_{2}$ n \Imp m $<$ n

lone:\\\tab{xxx} \Fol $\mbox{log}_{2}$ 1 = 0

lpot:\\\tab{xxx} \Fol $\mbox{log}_{2}$ 2$\hatsym$ n = n

lsucc-01:\\\tab{xxx} \Fol n $\neq$ 0 \Imp $\mbox{log}_{2}$(2 $*$ n + 1) = $\mbox{log}_{2}$ n + 1

ltwo-03:\\\tab{xxx} \Fol n $\neq$ 0 \Imp $\mbox{log}_{2}$(2 $*$ n) = $\mbox{log}_{2}$ n + 1

ltwo-04:\\\tab{xxx} \Fol $\mbox{log}_{2}$ 2 = 1

ltwo-05:\\\tab{xxx} \Fol n $<$ 2 $*$ 2$\hatsym$ $\mbox{log}_{2}$ n

lzer:\\\tab{xxx} \Fol $\mbox{log}_{2}$(m + 1) = 0 \Equiv m = 0

mult:\\\tab{xxx} \Fol (m $*$ \Var{m}{0}) $\hatsym$ n = m $\hatsym$ n $*$ \Var{m}{0} $\hatsym$ n

one:\\\tab{xxx} \Fol 2$\hatsym$ m = 1 \Equiv m = 0

one-01:\\\tab{xxx} \Fol 2$\hatsym$ 1 = 2

one-01-01:\\\tab{xxx} \Fol m $\hatsym$ 1 = m

one-02:\\\tab{xxx} \Fol 0 $\hatsym$ 1 = 0

pot-01:\\\tab{xxx}n $\neq$ 0 \Fol 2 $*$ 2$\hatsym$ n -1 = 2$\hatsym$ n

pot-mon:\\\tab{xxx}1 $<$ m \Fol m $\hatsym$ n $<$ m $\hatsym$ \Var{n}{0} \Equiv n $<$ \Var{n}{0}

pot-two:\\\tab{xxx} \Fol m $\hatsym$ 2 = m $*$ m

pot-zero:\\\tab{xxx} \Fol m $\neq$ 0 \Imp m $\hatsym$ n $\neq$ 0

pot2-def:\\\tab{xxx} \Fol 2$\hatsym$ m = 2 $\hatsym$ m

potex:\\\tab{xxx}n $\neq$ 0 \Fol \Ex m. 2$\hatsym$ m $\le$ n \And n $<$ 2$\hatsym$(m + 1)

potmon:\\\tab{xxx} \Fol 2$\hatsym$ m $<$ 2$\hatsym$ n \Equiv m $<$ n

rec:\\\tab{xxx} \Fol 2$\hatsym$(n + 1) = 2$\hatsym$ n + 2$\hatsym$ n

rec-01:\\\tab{xxx} \Fol n $\hatsym$ (m + 1) = n $\hatsym$ m $*$ n

succ-02:\\\tab{xxx} \Fol 2 $*$ 2$\hatsym$ m = 2$\hatsym$(m + 1)

succ-03:\\\tab{xxx} \Fol 2$\hatsym$ m = 2 $*$ n + 1 \Equiv m = 0 \And n = 0

two:\\\tab{xxx} \Fol m $\hatsym$ (2 $*$ n) = m $\hatsym$ n $*$ m $\hatsym$ n

two-pot-zero:\\\tab{xxx} \Fol 2 $\hatsym$ n $\neq$ 0

zero:\\\tab{xxx} \Fol 2$\hatsym$ n $\neq$ 0

zero-01:\\\tab{xxx} \Fol 0 $\hatsym$ n = 0 \Equiv n $\neq$ 0



\end{document}

