\documentclass[a4paper]{article}

\usepackage{latexsym,a4wide}

% The definition of \ifundefined is exercise 7.7 in the \TeX book
% \csname <Tokens> \endcsname is essentially \<Tokens>, i.e.
% some kind of evaluation. However, <Tokens> may contain tex-commands
% that are evaluated.
% \relax does nothing. Does this mean that \ifx\csname#1\endcsname
% is not evaluated when defining \ifundefined ?
% \expandafter evaluates everything after \ifx and then puts \ifx
% again in front.
% \ifndef{x}{y} tests whether x is defined. If yes, \x is carried out
% (the else part \csname#1\endcsname) otherwise y is the result.
% \ifdef{x} does \x if defined, nothing otherwise
\def\ifundefined#1{\expandafter\ifx\csname#1\endcsname\relax}
\newcommand{\ifndef}[2]{\ifundefined{#1}{#2}\else{\csname#1\endcsname}\fi}
\newcommand{\ifdef}[1]{\ifndef{#1}{}}

\newenvironment{fma}%
{\begin{equation}\begin{minipage}{0.85\linewidth}\raggedright}%
{\end{minipage}\end{equation}}

\newcommand{\udo}{$\langle$}
\newcommand{\udc}{$\rangle$}
\newcommand{\ubo}{$[$}
\newcommand{\ubc}{$]$}
\newcommand{\mkdia}[1]{\mbox{$\langle$#1$\rangle$}}
\newcommand{\mkbox}[1]{\mbox{$[$#1$]$}}
\newcommand{\tildesym}{\raisebox{-4pt}{\bf\~{}}}
\newcommand{\hatsym}{\mbox{\bf\^{} }}

\newcommand{\Fol}{\mbox{$\vdash\ $}}
\newcommand{\Not}{\mbox{$\neg\ $}}
\newcommand{\And}{\mbox{$\wedge\ $}}
\newcommand{\Or}{\mbox{$\vee\ $}}
\newcommand{\Imp}{\mbox{$\rightarrow\ $}}
\newcommand{\Equiv}{\mbox{$\leftrightarrow\ $}}
\newcommand{\All}{\mbox{$\forall\ $}}
\newcommand{\Ex}{\mbox{$\exists\ $}}

\newcommand{\tab}[1]{\mbox{$\phantom{\mbox{#1}}$}}
\newcommand{\tabx}[1]{\hspace*{#1ex}}
\newcommand{\tabif}{\tab{{\bf if}}}
\newcommand{\tabbe}{\tab{{\bf be}}}
\newcommand{\taball}{\mbox{$\phantom{\forall\ }$}}
\newcommand{\tabex}{\mbox{$\phantom{\exists\ }$}}
\newcommand{\taba}{\mbox{$\phantom{\wedge\ }$}}
\newcommand{\tabbo}{\mbox{$\phantom{(}$}}
\newcommand{\tabe}{\mbox{$\phantom{\leftrightarrow\ }$}}
\newcommand{\tabi}{\mbox{$\phantom{\rightarrow\ }$}}
\newcommand{\tabn}{\mbox{$\phantom{\neg\ }$}}
\newcommand{\tabo}{\mbox{$\phantom{\vee\ }$}}
\newcommand{\tabf}{\mbox{$\phantom{\vdash\ }$}}
\newcommand{\tabudo}{\mbox{$\phantom{\langle}$}}
\newcommand{\tabudc}{\mbox{$\phantom{\langle\ }$}}
\newcommand{\tabubo}{\mbox{$\phantom{[}$}}
\newcommand{\tabubc}{\mbox{$\phantom{]\ }$}}


\parindent0cm


\begin{document}
\raggedright
              
Spec theorems: 


{\bf Specification int-abs:}

intr,ax-01: 
 \Fol $\tildesym$ x = $\mbox{0}_{i}$ $\mbox{-}_{i}$ x



intr,ax-04: 
 \Fol y $\mbox{$<$}_{i}$ $\mbox{0}_{i}$ \Imp absi(y) = $\mbox{0}_{i}$ $\mbox{-}_{i}$ y



{\bf Specification int-lec:}

intr,anti: 
 \Fol x $\mbox{$\le$}_{i}$ y \Imp (y $\mbox{$\le$}_{i}$ x \Equiv x = y)



intr,ple-01: 
x $\mbox{$<$}_{i}$ y, 
$\mbox{x}_{0}$ $\mbox{$\le$}_{i}$ $\mbox{y}_{0}$
 \Fol x $\mbox{+}_{i}$ $\mbox{x}_{0}$ $\mbox{$<$}_{i}$ y $\mbox{+}_{i}$ $\mbox{y}_{0}$



intr,fle: 
 \Fol x $\mbox{$<$}_{i}$ y \And y $\mbox{$\le$}_{i}$ $\mbox{y}_{0}$ \Imp x $\mbox{$<$}_{i}$ $\mbox{y}_{0}$






Simplifier rules: 


{\bf Specification int-sub:}

intr,sub-zero: 
 \Fol x $\mbox{-}_{i}$ $\mbox{0}_{i}$ = x



intr,less-02: 
 \Fol x $\mbox{-}_{i}$ y $\mbox{$<$}_{i}$ z \Equiv x $\mbox{$<$}_{i}$ z $\mbox{+}_{i}$ y



intr,less-01: 
 \Fol x $\mbox{$<$}_{i}$ y $\mbox{-}_{i}$ z \Equiv x $\mbox{+}_{i}$ z $\mbox{$<$}_{i}$ y



intr,le-02: 
 \Fol x $\mbox{$\le$}_{i}$ y $\mbox{-}_{i}$ z \Equiv x $\mbox{+}_{i}$ z $\mbox{$\le$}_{i}$ y



intr,elim-sub: 
 \Fol z = x $\mbox{-}_{i}$ y \Equiv x = z $\mbox{+}_{i}$ y



intr,sub-sub: 
 \Fol x $\mbox{-}_{i}$ y $\mbox{-}_{i}$ z = x $\mbox{-}_{i}$ y $\mbox{+}_{i}$ z



intr,shift: 
 \Fol x $\mbox{+}_{i}$ (y $\mbox{-}_{i}$ z) = x $\mbox{+}_{i}$ y $\mbox{-}_{i}$ z



intr,eq: 
 \Fol x $\mbox{-}_{i}$ y = z \Equiv x = z $\mbox{+}_{i}$ y



intr,ax-01: 
 \Fol x $\mbox{+}_{i}$ (y $\mbox{-}_{i}$ x) = y



{\bf Specification intnat:}

nat2int-04: 
 \Fol n$\to$i(m) $\mbox{$<$}_{i}$ n$\to$i(n) \Equiv m $<$ n



ax-06: 
 \Fol n$\to$i(0) = $\mbox{0}_{i}$



nat2int-03: 
 \Fol n$\to$i(n + 1) = n$\to$i(n) $\mbox{+}_{i}$ $\mbox{1}_{i}$



nat2int-08: 
 \Fol \Not n$\to$i(n) $\mbox{$<$}_{i}$ $\mbox{0}_{i}$



labs: 
 \Fol i$\to$n(x) $<$ i$\to$n(y) \Equiv absi(x) $\mbox{$<$}_{i}$ absi(y)



{\bf Specification int-basic1:}

intr,pred: 
 \Fol x = y $\mbox{-1}_{i}$ \Equiv x $\mbox{+1}_{i}$ = y



intr,ls-pred: 
 \Fol x $\mbox{$<$}_{i}$ y $\mbox{-1}_{i}$ \Equiv x $\mbox{+1}_{i}$ $\mbox{$<$}_{i}$ y



intr,lf-03: 
 \Fol x $\mbox{$<$}_{i}$ y \And x = z \Imp z $\mbox{$<$}_{i}$ y



intr,lf-02: 
 \Fol x $\mbox{$<$}_{i}$ y \And y = z \Imp x $\mbox{$<$}_{i}$ z



intr,lst-01: 
 \Fol \Not x $\mbox{$<$}_{i}$ y \Imp (x $\neq$ y \Equiv y $\mbox{$<$}_{i}$ x)



intr,elim-pred: 
 \Fol x = y $\mbox{-1}_{i}$ \Equiv y = x $\mbox{+1}_{i}$



intr,ax-03: 
 \Fol \Not x $\mbox{$<$}_{i}$ x



intr,lf-01: 
 \Fol x $\mbox{$<$}_{i}$ y \And y $\mbox{$<$}_{i}$ z \Imp x $\mbox{+1}_{i}$ $\mbox{$<$}_{i}$ z



intr,ax-04: 
 \Fol x $\mbox{$<$}_{i}$ y \And y $\mbox{$<$}_{i}$ z \Imp x $\mbox{$<$}_{i}$ z



intr,ls-01: 
 \Fol x $\mbox{$<$}_{i}$ y \Imp \Not y $\mbox{$<$}_{i}$ x



{\bf Specification int-abs:}

intr,ax-02: 
 \Fol y $\mbox{$<$}_{i}$ $\mbox{0}_{i}$ \Imp sgn(y) = $\mbox{0}_{i}$ $\mbox{-1}_{i}$



intr,sgn+1: 
 \Fol $\mbox{0}_{i}$ $\mbox{$\le$}_{i}$ y \Imp sgn(y) = $\mbox{1}_{i}$



intr,neg-12: 
 \Fol $\tildesym$ x = $\tildesym$ y \Equiv x = y



intr,absls: 
 \Fol \Not absi(x) $\mbox{$<$}_{i}$ $\mbox{0}_{i}$



intr,neg-04: 
 \Fol $\tildesym$ $\mbox{0}_{i}$ = $\mbox{0}_{i}$



intr,neg-05: 
 \Fol $\tildesym$ x $\mbox{$<$}_{i}$ $\mbox{0}_{i}$ \Equiv $\mbox{0}_{i}$ $\mbox{$<$}_{i}$ x



intr,abs-16: 
 \Fol $\mbox{0}_{i}$ $\mbox{$<$}_{i}$ y \Imp absi(y) = y



intr,abs-06: 
 \Fol $\mbox{0}_{i}$ $\mbox{$<$}_{i}$ absi(x) \Equiv x $\neq$ $\mbox{0}_{i}$



intr,neg: 
 \Fol $\mbox{0}_{i}$ $\mbox{$<$}_{i}$ $\tildesym$ x \Equiv x $\mbox{$<$}_{i}$ $\mbox{0}_{i}$



intr,negle-13: 
 \Fol $\tildesym$ x $\mbox{$\le$}_{i}$ y \Equiv $\mbox{0}_{i}$ $\mbox{$\le$}_{i}$ x $\mbox{+}_{i}$ y



intr,neg-02: 
 \Fol $\tildesym$ $\tildesym$ x = x



intr,ax-04: 
 \Fol y $\mbox{$<$}_{i}$ $\mbox{0}_{i}$ \Imp absi(y) = $\mbox{0}_{i}$ $\mbox{-}_{i}$ y



intr,neg-06: 
 \Fol $\mbox{0}_{i}$ $\mbox{-}_{i}$ x = $\tildesym$ x



intr,negeq: 
 \Fol $\tildesym$ x = y \Equiv x $\mbox{+}_{i}$ y = $\mbox{0}_{i}$



intr,neg-15: 
 \Fol x $\mbox{+}_{i}$ $\tildesym$ y = x $\mbox{-}_{i}$ y



intr,abs-18: 
 \Fol absi(x) = x \Equiv $\mbox{0}_{i}$ $\mbox{$\le$}_{i}$ x



intr,ax-05: 
 \Fol \Not y $\mbox{$<$}_{i}$ $\mbox{0}_{i}$ \Imp absi(y) = y



intr,abs-02: 
 \Fol absi($\mbox{0}_{i}$) = $\mbox{0}_{i}$



intr,neg-03: 
 \Fol $\tildesym$ x $\mbox{+}_{i}$ x = $\mbox{0}_{i}$



{\bf Specification nat-lec:}

fle: 
 \Fol m $<$ n \And n $\le$ $\mbox{n}_{0}$ \Imp m $<$ $\mbox{n}_{0}$



fle-01: 
 \Fol m $\le$ n \And n $<$ $\mbox{n}_{0}$ \Imp m $<$ $\mbox{n}_{0}$



succ: 
 \Fol m +1 = m + 1



ax-02: 
 \Fol 0 $\neq$ 1



{\bf Specification nat-basic2:}

a: 
 \Fol (m + $\mbox{n}_{0}$) + $\mbox{n}_{1}$ = m + $\mbox{n}_{0}$ + $\mbox{n}_{1}$



c: 
 \Fol m + n = n + m



z-01: 
 \Fol m + n = 0 \Equiv m = 0 \And n = 0



{\bf Specification int-basic2:}

intr,zero-01: 
 \Fol x $\mbox{$<$}_{i}$ $\mbox{0}_{i}$ \And y $\mbox{$<$}_{i}$ $\mbox{0}_{i}$ \Imp x $\mbox{+}_{i}$ y $\mbox{$<$}_{i}$ $\mbox{0}_{i}$



intr,ls-02: 
 \Fol x $\mbox{$<$}_{i}$ x $\mbox{+}_{i}$ y \Equiv $\mbox{0}_{i}$ $\mbox{$<$}_{i}$ y



intr,ls: 
 \Fol x $\mbox{+}_{i}$ y $\mbox{$<$}_{i}$ y \Equiv x $\mbox{$<$}_{i}$ $\mbox{0}_{i}$



intr,eq: 
 \Fol x = x $\mbox{+}_{i}$ y \Equiv y = $\mbox{0}_{i}$



intr,ls-01: 
 \Fol x $\mbox{+}_{i}$ y $\mbox{$<$}_{i}$ x $\mbox{+}_{i}$ z \Equiv y $\mbox{$<$}_{i}$ z



intr,ax-03: 
 \Fol x $\mbox{+}_{i}$ y $\mbox{-1}_{i}$ = (x $\mbox{+}_{i}$ y)$\mbox{-1}_{i}$



intr,ax-01: 
 \Fol x $\mbox{+}_{i}$ $\mbox{0}_{i}$ = x



intr,zero-07: 
 \Fol x $\mbox{+}_{i}$ x = $\mbox{0}_{i}$ \Equiv x = $\mbox{0}_{i}$



intr,add-a: 
 \Fol x $\mbox{+}_{i}$ y $\mbox{+}_{i}$ z = (x $\mbox{+}_{i}$ y) $\mbox{+}_{i}$ z



intr,add-c: 
 \Fol x $\mbox{+}_{i}$ y = y $\mbox{+}_{i}$ x



intr,add-in: 
 \Fol x $\mbox{+}_{i}$ y = x $\mbox{+}_{i}$ z \Equiv y = z



{\bf Specification nat-basic1:}

ax-05: 
 \Fol \Not n $<$ n



{\bf Specification int-lec:}

intr,les: 
 \Fol x $\mbox{$<$}_{i}$ y \Imp (y $\mbox{$\le$}_{i}$ x $\mbox{+}_{i}$ $\mbox{1}_{i}$ \Equiv y = x $\mbox{+}_{i}$ $\mbox{1}_{i}$)



intr,zero: 
 \Fol $\mbox{1}_{i}$ $\mbox{+}_{i}$ $\mbox{$\tildesym$1}_{i}$ = $\mbox{0}_{i}$



intr,mone-02: 
 \Fol $\mbox{$\tildesym$1}_{i}$ $\mbox{$<$}_{i}$ $\mbox{0}_{i}$



intr,mone-07: 
 \Fol x = $\mbox{$\tildesym$1}_{i}$ \Equiv x $\mbox{+1}_{i}$ = $\mbox{0}_{i}$



intr,let: 
 \Fol y $\mbox{$\le$}_{i}$ $\mbox{y}_{0}$ \And $\mbox{y}_{0}$ $\mbox{$\le$}_{i}$ $\mbox{y}_{1}$ \Imp y $\mbox{$\le$}_{i}$ $\mbox{y}_{1}$



intr,bet: 
 \Fol $\mbox{0}_{i}$ $\mbox{$<$}_{i}$ x \Imp (x $\mbox{$\le$}_{i}$ $\mbox{1}_{i}$ \Equiv x = $\mbox{1}_{i}$)



intr,fle-01: 
 \Fol x $\mbox{$\le$}_{i}$ y \And y $\mbox{$<$}_{i}$ $\mbox{y}_{0}$ \Imp x $\mbox{$<$}_{i}$ $\mbox{y}_{0}$



intr,succ-01: 
 \Fol x $\mbox{+}_{i}$ $\mbox{1}_{i}$ $\mbox{$\le$}_{i}$ y \Equiv x $\mbox{$<$}_{i}$ y



intr,succ-02: 
 \Fol x $\mbox{$<$}_{i}$ y $\mbox{+}_{i}$ $\mbox{1}_{i}$ \Equiv x $\mbox{$\le$}_{i}$ y



intr,anti: 
 \Fol x $\mbox{$\le$}_{i}$ y \Imp (y $\mbox{$\le$}_{i}$ x \Equiv x = y)



intr,lels-04: 
 \Fol x $\mbox{$\le$}_{i}$ y \Imp (\Not \Not y $\mbox{$<$}_{i}$ x \Equiv false)



intr,lels-03: 
 \Fol x $\mbox{$<$}_{i}$ y \Imp (\Not \Not y $\mbox{$\le$}_{i}$ x \Equiv false)



intr,bet-01: 
 \Fol $\mbox{0}_{i}$ $\mbox{$\le$}_{i}$ x \Imp (x $\mbox{$<$}_{i}$ $\mbox{1}_{i}$ \Equiv x = $\mbox{0}_{i}$)



intr,one-01: 
 \Fol $\mbox{0}_{i}$ $\mbox{$<$}_{i}$ $\mbox{1}_{i}$



intr,ler: 
 \Fol x $\mbox{$\le$}_{i}$ x



intr,lels: 
 \Fol \Not x $\mbox{$<$}_{i}$ y \Equiv y $\mbox{$\le$}_{i}$ x



intr,fle: 
 \Fol x $\mbox{$<$}_{i}$ y \And y $\mbox{$\le$}_{i}$ $\mbox{y}_{0}$ \Imp x $\mbox{$<$}_{i}$ $\mbox{y}_{0}$



intr,lels-02: 
 \Fol x $\neq$ y \Imp (x $\mbox{$\le$}_{i}$ y \Equiv x $\mbox{$<$}_{i}$ y)



intr,lels-01: 
 \Fol \Not x $\mbox{$\le$}_{i}$ y \Equiv y $\mbox{$<$}_{i}$ x



intr,succ: 
 \Fol x $\mbox{+1}_{i}$ = x $\mbox{+}_{i}$ $\mbox{1}_{i}$








\end{document}

