\documentclass[a4paper]{article}

\usepackage{latexsym,a4wide,logicdefs,amssymb}

\parindent0cm


\begin{document}
\raggedright
              
unequal:\\ nat-basic2,eq-01: 
 \Fol m + n = m + \Var{n}{0} \Equiv n = \Var{n}{0}



nat-basic2,oz: 
 \Fol m + 1 $\neq$ 0



nat-basic2,a: 
 \Fol (m + \Var{n}{0}) + \Var{n}{1} = m + \Var{n}{0} + \Var{n}{1}



nat-basic2,c: 
 \Fol m + n = n + m



nat-basic2,succ: 
 \Fol m +1 = m + 1



list-data,size-01: 
 \Fol \# [] = 0



list-data,l: 
 \Fol \# x = 0 \Equiv x = []



\bigskip

two:\\ 

\bigskip

split-rest:\\ nat,lep: 
 \Fol m $\le$ m + n



nat-basic2,eq-01: 
 \Fol m + n = m + \Var{n}{0} \Equiv n = \Var{n}{0}



nat,elim-sub: 
n $\le$ m
 \Fol \Var{n}{0} = m - n \Equiv m = \Var{n}{0} + n



nat-basic1,ref-1: 
 \Fol \Not n $<$ n



nat,fle-01: 
 \Fol m $\le$ n \And n $<$ \Var{n}{0} \Imp m $<$ \Var{n}{0}



nat-basic1,f: 
 \Fol m $<$ n \Imp n $\neq$ 0



nat,fle: 
 \Fol m $<$ n \And n $\le$ \Var{n}{0} \Imp m $<$ \Var{n}{0}



nat,lels-01: 
 \Fol \Not m $\le$ n \Equiv n $<$ m



nat,ls-03: 
\Var{n}{0} $\le$ n
 \Fol n - \Var{n}{0} $\le$ m \Equiv n $\le$ m + \Var{n}{0}



nat-basic2,l-02: 
 \Fol \Not m + n $<$ m



nat-basic2,a: 
 \Fol (m + \Var{n}{0}) + \Var{n}{1} = m + \Var{n}{0} + \Var{n}{1}



nat-basic2,c: 
 \Fol m + n = n + m



\bigskip

split-first:\\ nat-basic1,one-01: 
 \Fol m $<$ 1 \Equiv m = 0



nat,eq-02: 
n $\le$ m
 \Fol (m - n) + \Var{n}{0} = \Var{n}{1} \Equiv m + \Var{n}{0} = n + \Var{n}{1}



nat,lep: 
 \Fol m $\le$ m + n



nat-basic1,ref-1: 
 \Fol \Not n $<$ n



nat,fle-01: 
 \Fol m $\le$ n \And n $<$ \Var{n}{0} \Imp m $<$ \Var{n}{0}



nat,fle: 
 \Fol m $<$ n \And n $\le$ \Var{n}{0} \Imp m $<$ \Var{n}{0}



nat,lels: 
 \Fol \Not m $<$ n \Equiv n $\le$ m



nat-basic1,lf-01: 
 \Fol m $<$ n \And n = \Var{n}{0} \Imp m $<$ \Var{n}{0}



nat,le-one: 
 \Fol m $\le$ n + 1 \And n $<$ \Var{n}{0} \Imp m $\le$ \Var{n}{0}



nat-basic2,a: 
 \Fol (m + \Var{n}{0}) + \Var{n}{1} = m + \Var{n}{0} + \Var{n}{1}



nat-basic2,c: 
 \Fol m + n = n + m



nat-basic1,f: 
 \Fol m $<$ n \Imp n $\neq$ 0



nat,leprf: 
 \Fol m $\le$ m - 1 \Imp m = 0



nat,lez: 
 \Fol 0 $\le$ m



nat-basic1,less-1: 
 \Fol \Not n $<$ 0



nat,pred-03: 
 \Fol n -1 = n - 1



nat,lels-01: 
 \Fol \Not m $\le$ n \Equiv n $<$ m



list-data,size-01: 
 \Fol \# [] = 0



nat,lez-01: 
 \Fol m $\le$ 0 \Equiv m = 0



list-data,l: 
 \Fol \# x = 0 \Equiv x = []



\bigskip

rewlem:\\ 

\bigskip

rest-01:\\ list-data,elim-list-c: 
x $\neq$ []
 \Fol a = x.first \And y = x.rest \Equiv x = a + y



\bigskip

rest:\\ list-data,sel-2: 
 \Fol (a + x).rest = x



\bigskip

onein:\\ list-data,lf-01: 
 \Fol \# x = 1 \Equiv x = x.first + []



list-data,elim-list-c: 
x $\neq$ []
 \Fol a = x.first \And y = x.rest \Equiv x = a + y



\bigskip

one-01:\\ 

\bigskip

one:\\ 

\bigskip

ni:\\ 

\bigskip

neq-09:\\ 

\bigskip

neq-07:\\ 

\bigskip

neq-06:\\ 

\bigskip

neq-05:\\ 

\bigskip

neq-04:\\ 

\bigskip

neq-03:\\ 

\bigskip

neq-02:\\ 

\bigskip

neq-01:\\ 

\bigskip

neq:\\ 

\bigskip

less-append:\\ list-data,less-02: 
 \Fol \Var{x}{0} $<$ a + x \Equiv \Var{x}{0} = x \Or \Var{x}{0} $<$ x



\bigskip

len-last-rest:\\ nat-basic2,eq-01: 
 \Fol m + n = m + \Var{n}{0} \Equiv n = \Var{n}{0}



nat-basic2,a: 
 \Fol (m + \Var{n}{0}) + \Var{n}{1} = m + \Var{n}{0} + \Var{n}{1}



nat-basic2,c: 
 \Fol m + n = n + m



list-data,elim-list-c: 
x $\neq$ []
 \Fol a = x.first \And y = x.rest \Equiv x = a + y



\bigskip

len-06:\\ nat-basic2,eq-01: 
 \Fol m + n = m + \Var{n}{0} \Equiv n = \Var{n}{0}



nat-basic2,a: 
 \Fol (m + \Var{n}{0}) + \Var{n}{1} = m + \Var{n}{0} + \Var{n}{1}



nat-basic2,c: 
 \Fol m + n = n + m



\bigskip

len-05:\\ list-data,size-02: 
 \Fol \#(a + x) = (\# x)+1



nat-basic2,succ: 
 \Fol m +1 = m + 1



nat-basic2,eq-01: 
 \Fol m + n = m + \Var{n}{0} \Equiv n = \Var{n}{0}



nat-basic2,a: 
 \Fol (m + \Var{n}{0}) + \Var{n}{1} = m + \Var{n}{0} + \Var{n}{1}



nat-basic2,c: 
 \Fol m + n = n + m



\bigskip

len-04:\\ nat-basic2,z: 
 \Fol 0 + m = m



list-data,size-01: 
 \Fol \# [] = 0



nat,lels-01: 
 \Fol \Not m $\le$ n \Equiv n $<$ m



nat,le-num-02: 
\Var{n}{0} $<$ n
 \Fol m + (* n) $\le$ \Var{m}{0} + (* \Var{n}{0}) \Equiv m + (n - \Var{n}{0}) $\le$ \Var{m}{0}



nat,lep-02: 
 \Fol m + n $\le$ m + \Var{n}{0} \Equiv n $\le$ \Var{n}{0}



nat,lep-01: 
 \Fol m + n $\le$ m \Equiv n = 0



nat-basic2,oz: 
 \Fol m + 1 $\neq$ 0



nat-basic2,a: 
 \Fol (m + \Var{n}{0}) + \Var{n}{1} = m + \Var{n}{0} + \Var{n}{1}



nat-basic2,c: 
 \Fol m + n = n + m



nat,lels: 
 \Fol \Not m $<$ n \Equiv n $\le$ m



\bigskip

len-03:\\ nat-basic1,ref-1: 
 \Fol \Not n $<$ n



nat,lels: 
 \Fol \Not m $<$ n \Equiv n $\le$ m



nat-basic2,l-02: 
 \Fol \Not m + n $<$ m



nat-basic2,a: 
 \Fol (m + \Var{n}{0}) + \Var{n}{1} = m + \Var{n}{0} + \Var{n}{1}



nat-basic2,c: 
 \Fol m + n = n + m



list-data,l: 
 \Fol \# x = 0 \Equiv x = []



nat-basic1,f: 
 \Fol m $<$ n \Imp n $\neq$ 0



\bigskip

len-02:\\ list-data,lf-01: 
 \Fol \# x = 1 \Equiv x = x.first + []



list-data,sel-1: 
 \Fol (a + x).first = a



list-data,f: 
 \Fol a + x = a + y \Equiv x = y



\bigskip

len-01:\\ nat-basic2,eq-01: 
 \Fol m + n = m + \Var{n}{0} \Equiv n = \Var{n}{0}



nat-basic2,oz: 
 \Fol m + 1 $\neq$ 0



nat-basic2,a: 
 \Fol (m + \Var{n}{0}) + \Var{n}{1} = m + \Var{n}{0} + \Var{n}{1}



nat-basic2,c: 
 \Fol m + n = n + m



list-data,size-01: 
 \Fol \# [] = 0



list-data,l: 
 \Fol \# x = 0 \Equiv x = []



\bigskip

len:\\ nat-basic2,eq-01: 
 \Fol m + n = m + \Var{n}{0} \Equiv n = \Var{n}{0}



nat-basic2,succ: 
 \Fol m +1 = m + 1



list-data,size-01: 
 \Fol \# [] = 0



nat-basic2,z: 
 \Fol 0 + m = m



nat-basic2,a: 
 \Fol (m + \Var{n}{0}) + \Var{n}{1} = m + \Var{n}{0} + \Var{n}{1}



nat-basic2,c: 
 \Fol m + n = n + m



\bigskip

lasttwo:\\ 

\bigskip

lastoc-rew:\\ 

\bigskip

lastoc:\\ 

\bigskip

lastdiv-rew:\\ 

\bigskip

lastdiv:\\ 

\bigskip

last-01:\\ 

\bigskip

last:\\ 

\bigskip

isin-01:\\ 

\bigskip

isin:\\ 

\bigskip

ins-01:\\ 

\bigskip

ins:\\ 

\bigskip

inex-03:\\ 

\bigskip

inex-02:\\ 

\bigskip

inex-01:\\ 

\bigskip

inex:\\ 

\bigskip

inapp-14:\\ 

\bigskip

inapp-13:\\ 

\bigskip

inapp-12:\\ 

\bigskip

inapp-11:\\ 

\bigskip

inapp-10:\\ 

\bigskip

inapp-09:\\ 

\bigskip

inapp-08:\\ 

\bigskip

inapp-07:\\ 

\bigskip

inapp-06:\\ 

\bigskip

inapp-05:\\ 

\bigskip

inapp-04:\\ 

\bigskip

inapp-03:\\ 

\bigskip

inapp-02:\\ 

\bigskip

inapp-01:\\ 

\bigskip

inapp:\\ list-data,elim-list-c: 
x $\neq$ []
 \Fol a = x.first \And y = x.rest \Equiv x = a + y



\bigskip

in-rec:\\ list-data,elim-list-c: 
x $\neq$ []
 \Fol a = x.first \And y = x.rest \Equiv x = a + y



\bigskip

in-last-rest:\\ 

\bigskip

in-empty:\\ 

\bigskip

in-append:\\ 

\bigskip

in-17:\\ 

\bigskip

in-16:\\ 

\bigskip

in-15:\\ 

\bigskip

in-14:\\ 

\bigskip

in-13:\\ 

\bigskip

in-12:\\ 

\bigskip

in-11:\\ 

\bigskip

in-10:\\ 

\bigskip

in-09:\\ list-data,elim-list-c: 
x $\neq$ []
 \Fol a = x.first \And y = x.rest \Equiv x = a + y



\bigskip

in-08:\\ list-data,elim-list-c: 
x $\neq$ []
 \Fol a = x.first \And y = x.rest \Equiv x = a + y



\bigskip

in-07:\\ list-data,elim-list-c: 
x $\neq$ []
 \Fol a = x.first \And y = x.rest \Equiv x = a + y



\bigskip

in-06:\\ 

\bigskip

in-01:\\ 

\bigskip

in:\\ 

\bigskip

if-in:\\ 

\bigskip

fr:\\ list-data,fr-02: 
 \Fol x $\neq$ [] \Imp x.first + x.rest = x



\bigskip

firstrest:\\ list-data,elim-list-c: 
x $\neq$ []
 \Fol a = x.first \And y = x.rest \Equiv x = a + y



\bigskip

firstoc-rew:\\ 

\bigskip

firstoc:\\ 

\bigskip

firsteq-01:\\ list-data,elim-list-c: 
x $\neq$ []
 \Fol a = x.first \And y = x.rest \Equiv x = a + y



\bigskip

firsteq:\\ list-data,elim-list-c: 
x $\neq$ []
 \Fol a = x.first \And y = x.rest \Equiv x = a + y



\bigskip

first-app:\\ list-data,elim-list-c: 
x $\neq$ []
 \Fol a = x.first \And y = x.rest \Equiv x = a + y



list-data,elim-1: 
 \Fol x $\neq$ [] \Imp (a = x.first \And \Var{x}{0} = x.rest \Equiv x = a + \Var{x}{0})



\bigskip

first-02:\\ list-data,elim-list-c: 
x $\neq$ []
 \Fol a = x.first \And y = x.rest \Equiv x = a + y



\bigskip

first-01:\\ list-data,elim-list-c: 
x $\neq$ []
 \Fol a = x.first \And y = x.rest \Equiv x = a + y



\bigskip

first:\\ list-data,sel-1: 
 \Fol (a + x).first = a



\bigskip

eq-05:\\ 

\bigskip

eq-04:\\ 

\bigskip

eq-03:\\ 

\bigskip

eq-02:\\ 

\bigskip

eq-01:\\ 

\bigskip

eq:\\ 

\bigskip

elim-first:\\ 

\bigskip

e-04:\\ nat-basic2,c: 
 \Fol m + n = n + m



nat-basic2,a: 
 \Fol (m + \Var{n}{0}) + \Var{n}{1} = m + \Var{n}{0} + \Var{n}{1}



list-data,l: 
 \Fol \# x = 0 \Equiv x = []



nat-basic2,z-01: 
 \Fol m + n = 0 \Equiv m = 0 \And n = 0



nat-basic2,eq: 
 \Fol m = m + n \Equiv n = 0



\bigskip

e-03:\\ 

\bigskip

e-02:\\ 

\bigskip

e-01:\\ list-data,disj-1: 
 \Fol [] $\neq$ a + x



\bigskip

e:\\ list-data,disj-1: 
 \Fol [] $\neq$ a + x



\bigskip

c-09:\\ 

\bigskip

c-08:\\ list-data,sel-1: 
 \Fol (a + x).first = a



\bigskip

c-07:\\ list-data,sel-2: 
 \Fol (a + x).rest = x



\bigskip

c-06:\\ list-data,inj-1: 
 \Fol a + x = \Var{a}{0} + \Var{x}{0} \Equiv a = \Var{a}{0} \And x = \Var{x}{0}



\bigskip

c-05:\\ 

\bigskip

c-04:\\ list-data,inj-1: 
 \Fol a + x = \Var{a}{0} + \Var{x}{0} \Equiv a = \Var{a}{0} \And x = \Var{x}{0}



\bigskip

c-03:\\ list-data,f: 
 \Fol a + x = a + y \Equiv x = y



list-data,inj-1: 
 \Fol a + x = \Var{a}{0} + \Var{x}{0} \Equiv a = \Var{a}{0} \And x = \Var{x}{0}



\bigskip

c-02:\\ list-data,elim-list-c: 
x $\neq$ []
 \Fol a = x.first \And y = x.rest \Equiv x = a + y



\bigskip

c-01:\\ 

\bigskip

c:\\ list-data,f: 
 \Fol a + x = a + y \Equiv x = y



\bigskip

app-09:\\ 

\bigskip

app-08:\\ 

\bigskip

app-07:\\ 

\bigskip

app-06:\\ 

\bigskip

app-05:\\ 

\bigskip

app-04:\\ 

\bigskip

app-03:\\ 

\bigskip

app-02-ant:\\ 

\bigskip

app-02:\\ 

\bigskip

app-01:\\ list-data,inj-1: 
 \Fol a + x = \Var{a}{0} + \Var{x}{0} \Equiv a = \Var{a}{0} \And x = \Var{x}{0}



\bigskip

app:\\ 

\bigskip

a:\\ list-data,f: 
 \Fol a + x = a + y \Equiv x = y



\bigskip

Noassoc:\\ 

\bigskip



\end{document}

